rfsfun.v
@@ -2,6 +2,23 @@ From mathcomp Require Import ssreflect ssrfun ssrbool ssrnat seq fintype choice.
 From mathcomp Require Import eqtype fingraph path order tuple path finmap finfun finset. 
 From event_struct Require Import utilities.
 
+(******************************************************************************)
+(* This file contains the definitions of:                                     *)
+(*           rfsfun dflt dom r  == that a function that defined on subset of  *)
+(*                            dom and behaives like dflt function out of it's *)
+(*                            domain. Also we requre that it's restriction    *)
+(*                            on dom (as a relation) should be a subrelation  *)
+(*                            of r                                            *)
+(*           rfsfun_i rr' ffr == if we've got `ffr : rfsfun dflt dom r` and   *)
+(*                           rr' -- proof that r x (f x) implies r' x (f x)   *)
+(*                           on all elements from dom than we can obtain a    *)
+(*                           new rfsfun of type `rfsfun dflt dom r'`          *)
+(*           add_rsfufn fd a pf ffr == if we have some                        *)
+(*                                 `ffr : rfsfun dflt dom r` and pf -- proof  *)
+(*                                 of `r fd a` we can extand out ffr on one   *)
+(*                                 element fd and bind in to a                *)
+(******************************************************************************)
+
 (* ************************************************************************* *)
 (*     fsfun with relation                                                   *)
 (* ************************************************************************* *)
@@ -14,11 +31,11 @@ Local Coercion fsval: fset_sub_type >-> Choice.sort.
 Open Scope fset_scope.
 
 Structure rfsfun {S : choiceType} {T : eqType}
-  (dflt : S -> T) (dom : {fset S}) (r : S -> T -> bool) := 
+  (dflt : S -> T) (dom : seq S) (r : S -> T -> bool) := 
   Rfsfun {
-  f :> {fsfun S -> T for dflt};
-  #[canonical(false)] dom_f : finsupp f `<=` dom;
-  #[canonical(false)] dep : [forall x : dom, r x (f x)]
+  f                         :> {fsfun S -> T for dflt};
+  #[canonical(false)] dom_f : [forall x : finsupp f, (fsval x) \in dom];
+  #[canonical(false)] dep   : all (fun x => r x (f x)) dom;
 }.
 (* For example if we take                                                    *)
 (* dom := 0,...,n                                                            *)
@@ -32,7 +49,7 @@ Structure rfsfun {S : choiceType} {T : eqType}
 Section rfsfunProperties.
 
 Context {n : nat} {S : choiceType} {T : eqType}
-  {dflt : S -> T} {dom : {fset S}} {r : S -> T -> bool}.
+  {dflt : S -> T} {dom : seq S} {r : S -> T -> bool}.
 Variable t : rfsfun dflt dom r.
 
 (* ************************************************************************* *)
@@ -46,12 +63,12 @@ Proof.
   move /negP=> D.
   apply/eqP; rewrite -memNfinsupp; apply/negP.
   move=> I; apply/D; move: I.
-  by rewrite -2!fsub1set=> /fsubset_trans/(_ (dom_f t)).
+  by move/forallP: (dom_f t)=> /swap L /(_ [` L]).
 Qed.
 
 (* for each `x \in dom` for `fun_of` function must holds such axiom *)
 Lemma axiom_rfsfun x : x \in dom -> r x (t x).
-Proof. by move/forallP: (dep t)=> /swap L /(_ [` L]). Qed.
+Proof. by move/allP: (dep t)=> /apply. Qed.
 
 End FunOfrffun.
 
@@ -68,30 +85,44 @@ Open Scope fset_scope.
 
 Notation add_f := ([fsfun t with fd |-> a]).
 
-Lemma dep_add : r fd a -> [forall x : fd |` dom, r x (add_f x)].
+Lemma dep_add : r fd a -> all (fun x => r x (add_f x)) (fd :: dom).
 Proof.
-  move=> ?. apply/forallP=> [[/= x /fset1UP[->|/axiom_rfsfun]]].
-  - by rewrite fsfun_with.
-  rewrite fsfun_withE; by case: ifP=> [/eqP->|].
+  move=> ?; apply/allP=> ?.
+  rewrite ?inE fsfun_withE.
+  by case: ifP=> /= [/eqP-> //| ? /(allP (dep t))].
 Qed.
 
-Lemma finsupp_add_f: finsupp add_f `<=` fd |` dom.
+Lemma finsupp_add_f: [forall x : finsupp add_f, (fsval x) \in fd :: dom].
 Proof.
-  rewrite finsupp_with; case: ifP=> ?.
-  - exact/(fsubset_trans (fsubD1set _ _))/(fsubset_trans (dom_f t))/fsubsetU1.
-  rewrite ![fd |` _]fsetUC; exact: (fsetSU _ (dom_f t)).
+  apply/forallP=> [[/= ?]]. 
+  rewrite finsupp_with /= ?inE.
+  case: ifP=> [? /fsetD1P[? L]|? /fset1UP[->| L]];
+  by rewrite ?eq_refl // (forallP (dom_f t) [` L]).
 Qed.
 
 End AddingElement.
 
+Context {r' : S -> T -> bool} 
+        (rr' : all (fun x => r x (t x) ==> r' x (t x)) dom).
+
+Lemma dep_r': all (fun x => r' x (t x)) dom.
+Proof.
+  apply/allP.
+  by move/allP: rr'=> H ? /dup I /H /implyP /(_ (allP (dep t) _ I)).
+Qed.
+
+Definition rfsfun_impl := Rfsfun (dom_f t) (dep_r').
+
 End rfsfunProperties.
 
 Definition add_rfsfun 
-  {S : choiceType} {T : eqType} {dflt dom fd a} {r : S -> T -> bool}
+  (S : choiceType) (T : eqType) dflt dom (r : S -> T -> bool) fd a
   (rafd : r fd a) (t : @rfsfun S T dflt dom r) :=
   Rfsfun (finsupp_add_f t) (dep_add t rafd).
 
-Notation "pf ':::' t" := (add_rfsfun pf t) (at level 20).
+Arguments add_rfsfun {_ _ _ _ _}.
+
+Notation "pf ':::' t" := (add_rfsfun _ _ pf t) (at level 20).
 
 Lemma fun_of_add_rffun 
   (S : choiceType) (T : eqType)
